\subsection{Jätkuedastussemantikas}

\footnotesize
\(
S'_{gs} \llbracket
\text{while\ } x \neq y \text{\ do\ }
  (\text{if\ } x \leq y
  \text{\ then\ } y := y - x \text{\ else\ } x := x - y )
\rrbracket
= FIX \ G,
\\
\text{kus} \ G(g) c = cond(B \llbracket x \neq y \rrbracket, 
S'_{cs} \llbracket \text{if\ } x \leq y \text{\ then\ } y := y - x
\text{\ else\ } x := x - y \rrbracket(g c),
c
)
\\
\)

Reegli \(S'_{cs} \llbracket S \rrbracket c = c \circ S_{ds} \llbracket S \rrbracket \) (raamatus punkt 4.74)
järgi võib tuletada:

\( \\
(FIX \ G) c \ s = (c \circ (FIX \ F))(s) = c( FIX \ F \ s) \\
\\
= \left \{ \begin{array}{l l}
  c ( s[y \mapsto \frac{sy}{i}][x \mapsto \frac{sx}{j} ]) & \quad \text{kui}\ (i * sx = j * sy) \wedge (i \neq j) \\
  c s & \quad \text{kui}\ sx = sy \\
\end{array} \right.
\\
\)

